simplify proof: remove next_call

theories/elpi_next.v
@@ -124,149 +124,70 @@ Section next_callS.
   Variable p : program.
   Variable u : Unif.
 
-  Fixpoint next_callS fv s A := 
-    match A with
-    | OK | Dead | KO | TA cut => (fv, A)
-    | TA (call t) => (backchain u p fv s t)
-    | Or A sx B => if is_dead A then 
-        let X := (next_callS fv s B) in (X.1, Or A sx X.2) else 
-        let X := (next_callS fv s A) in (X.1, Or X.2 sx B)
-    | And A B0 B =>
-      if success A then 
-        let X := (next_callS fv s B) in (X.1, And A B0 X.2) else
-        let X := (next_callS fv s A) in (X.1, And X.2 B0 B)
-  end.
-
-  Lemma is_dead_next_callS s fv A: is_dead (next_callS fv s A).2 = is_dead A.
-  Proof.
-    elim: A => //=.
-    - move=> []// c; rewrite/backchain; case: F => [? [|[]]]//.
-    - move=> A HA s1 B HB; case: ifP => dA/=.
-        rewrite dA HB//.
-      by rewrite HA dA.
-    - move=> A HA B0 B HB; case: ifP => sA//=.
-  Qed.
-
-  Lemma next_callS_valid fv s A B: 
-    valid_tree A -> failed A = false -> next_callS s fv A = B -> valid_tree B.2.
-  Proof.
-    move=> ++ <-; clear B.
-    elim: A s => //=.
-    - by move=> []// c s _ _; rewrite valid_tree_backchain.
-    - move=> A HA s1 B HB s2.
-      case: ifP => [dA vB fB|dA /andP[vA bB] fA]/=.
-        by rewrite dA HB.
-      by rewrite bB HA// bbOr_valid// if_same.
-    - move=> A HA B0 B HB s /andP[vA].
-      case fA: failed => //=.
-      case: ifP => /=[sA vB fB|sA /eqP->{B HB} _].
-        move: (HB s vB fB) => {HA HB} vB'.
-        rewrite vA vB' sA//.
-      by rewrite HA//= eqxx valid_tree_big_and if_same.
-  Qed.
-
-  Lemma failed_next_callS fv s A sx bt sz t gl a ign:
-    valid_tree A -> failed A = false ->
-      t2l A sx bt = (sz, ((call t), ign) :: gl) :: a -> failed (next_callS s fv A).2.
-  Proof.
-    elim: A sx bt gl a ign => //=.
-    - move=> []// *; rewrite failed_big_or//.
-    - move=> A HA s1 B HB sx bt gl a ign; case: ifP => [dA vB fB|dA /andP[vA bB] fA].
-        rewrite t2l_dead//.
-        case X: t2l => [|[s' [|[[|g'] al] gs']] rs]//[?????]; subst.
-        by move=> /=; rewrite dA; apply: HB  X.
-      set X:= t2l B _ _.
-      have [sg[g [gs H]]] := failed_t2l vA fA sx X.
-      rewrite H; case: g H => //-[[|g a']gs']// H [?????]; subst => /=.
-      rewrite /= (HA _ _ _ _ _ _ _ H)//.
-      by rewrite is_dead_next_callS dA.
-    - move=> A HA B0 B HB sx bt gl a ign /andP[vA].
-      case fA: failed => //=.
-      case: ifP => /=[sA vB fB|sA/eqP->{B HB} _].
-        rewrite (success_t2l empty)//sA fA/=.
-        rewrite make_lB01_empty2/=.
-        set ml:= make_lB0 _ _.
-        have [s2'[x[xs H1]]] := [elaborate failed_t2l vB fB (get_substS sx A) (ml ++ bt)].
-        rewrite H1/=.
-        case: x H1 => //-[[|g'] as'] gs'//= H1 [?????]; subst.
-        by apply: HB H1.
-      have [s2'[x[xs H]]] := failed_t2l vA fA sx bt.
-      rewrite H/= t2l_big_and => -[?+?]; subst.
-      case: x H => //=.
-        move=> H.
-        exfalso.
-        by apply: s2l_empty_hdF H.
-      move=> [[|g]]//= c' gs H [??]; subst.
-      rewrite (HA _ _ _ _ _ _ _ H)//.
-  Qed.
-
   Lemma next_callS_s2l fv A s3 s1 bt t gl a ign:
-    let X := (next_callS fv s1 A) in
+    let X := step u p fv s3 A in
     let F := F u p fv t s1 in
     failed A = false -> valid_tree A ->
       clean_ca bt (t2l A s3 bt) = (s1, (call t, ign) :: gl) ::: a ->
-        [/\ F.1 = X.1,
+        [/\
         clean_ca bt (t2l X.2 s3 bt) = 
           (save_alts a gl (aa2gs F.2) ++ a) &
-        step u p fv s3 A = 
-          (X.1, Expanded, X.2)].
+        X = (F.1, Expanded, X.2)].
   Proof.
-    elim: A s3 bt s1 t gl a ign => //=.
-    - move=> []// c s3 bt s1 c1 gl a ign _ _ [?????]; subst.
+    move=> /=.
+    elim: A s3 bt s1 t gl a ign fv => //=.
+    - move=> []// c s3 bt s1 c1 gl a ign fv _ _ [?????]; subst.
       rewrite push.
       rewrite what_I_want; last by rewrite valid_tree_backchain.
-      rewrite cats0; split => //.
-        by rewrite/backchain push//.
-      rewrite/backchain !push.
-      case B: F => [? [|[sx x]xs]]//=.
-      rewrite add_ca_deep_empty1 cat0s.
-      have:= @s2l_big_or sx sx (premises x) xs no_alt no_goals.
-      rewrite make_lB0_empty2/= add_ca_deep_empty1 cat0s.
-      move=> <-//.
-    - move=> A HA s B HB s1 bt s2 t gl a ign.
+      rewrite/backchain !push/=.
+      case X: F => [fv' [|[s0 r0] rs]]//=.
+      rewrite cat0s cats0 add_ca_deep_empty1.
+      have:= @s2l_big_or s1 s0 (premises r0) rs no_alt no_goals.
+      rewrite make_lB0_empty2/= add_ca_deep_empty1 cat0s => <-//.
+    - move=> A HA s B HB s1 bt s2 t gl a ign fv.
+      rewrite !push.
       case: ifP => [dA fB vB|dA fA /andP[vA bB]]/=.
         rewrite !(t2l_dead dA)//=cat0s.
         rewrite clean_ca_add_ca1 => X.
         rewrite -(@clean_ca_nil (t2l B s [::])) in X.
-        have [He {}HB H]:= HB s no_alt _ _ _ _ _ fB vB X.
+        have [{}HB H]:= HB s no_alt _ _ _ _ _ fv fB vB X.
         rewrite clean_ca_nil in HB.
-        by rewrite HB/= clean_ca_add_ca1 H//= cat0s//.
-      have [s'[x[xs H]]] := [elaborate failed_t2l vA fA s1 (t2l B s nilC)].
+        by rewrite H HB/= cat0s clean_ca_add_ca1//.
+      have [s'[x[xs H]]] := failed_t2l vA fA s1 (t2l B s [::]).
       rewrite H/=; case: x H => //-[[|g] ca] gs// H [?????]; subst.
-      have {HA HB} := HA s1 (t2l B s no_alt) _ _ _ _ _ fA vA.
-      rewrite H/= => /(_ _ _ _ _ _ erefl) [He + H1].
-      fNilA.
-      rewrite what_I_want ?(next_callS_valid _ _ erefl)//!clean_ca_add_ca1.
-      rewrite H1 => Hz; repeat split.
-        by rewrite He.
+      have {HA HB} := HA s1 (t2l B s no_alt) _ _ _ _ _ fv fA vA.
+      rewrite H/= => /(_ _ _ _ _ _ erefl) [+ H1].
+      rewrite H1/= seq2alts_cat !seq2altsK.
+      rewrite (what_I_want (valid_tree_step vA erefl)) !clean_ca_add_ca1/=.
+      move=> Hz; repeat split.
       have [?] := s2l_Expanded_call vA H1 H; subst.
-      move: He.
-      case X: F => [?[|[sz z]zs]] /= He [?]; subst.
+      move: Hz H1.
+      case X: F => [?[|[sz z]zs]] /= Hz H1 [?]; subst.
         by move=> [Hm Hn]; rewrite Hn/=cat0s//.
       move=> [Hm Hn]; rewrite Hn/=.
       rewrite clean_ca_goals_add_ca_goal1.
       by rewrite !catA.
-    - move=> A HA B0 B HB s1 bt s2 t gl a ign.
+    - move=> A HA B0 B HB s1 bt s2 t gl a ign fv.
       case fA: failed => //= + /andP[vA].
-      case: ifP => /=[sA fB vB |sA _ /eqP-> {B HB}].
+      rewrite !push/=.
+      case eA: step => [[fvA rA] A']/=.
+      case eB: step => [[fvB rB] B']/=.
+      case: ifP => /=[sA fB vB |sA _ /eqP?]; subst.
+        move: eA; rewrite success_step// => -[???]; subst => /=.
         rewrite (success_t2l empty)//=.
-        (* move/orPT: bB => []bB; last first.
-          rewrite base_and_ko_t2l//= make_lB01_empty2 => H.
-          have /={HA HB}[HB H1] := HB _ _ _ _ _ _ _ fB vB H.
-          rewrite success_step//H1/= make_lB01_empty2 HB//.
-        have [h H]:= base_and_t2l bB. *)
         rewrite make_lB01_empty2/=.
         rewrite clean_ca_cat.
         set ml:= make_lB0 _ _.
-        have [s2'[x[xs H1]]] := [elaborate failed_t2l vB fB (get_substS s1 A) (ml ++ bt)].
+        have [s2'[x[xs H1]]] := [elaborate failed_t2l vB fB (get_substS s1 A') (ml ++ bt)].
         rewrite H1/=.
         case: x H1 => [|[[|c']ca'] gs]// H1 [?????]; subst.
-        have /={HA HB} := HB (get_substS s1 A) (ml ++ bt) _ _ _ _ _ fB vB _.
+        have /={HA HB} := HB (get_substS s1 A') (ml ++ bt) _ _ _ _ _ fvA fB vB.
         move=> /(_ _ IsList_alts).
-        rewrite H1/= =>  // /(_ _ _ _ _ _ erefl) [He {}HB H2].
-        rewrite success_step//=.
-        rewrite H2 make_lB01_empty2; repeat split => //.
-        have [?] := s2l_Expanded_call vB H2 H1; subst.
+        rewrite H1/= =>  // /(_ _ _ _ _ _ erefl) [{}HB].
+        rewrite eB => -[??]; subst => /=.
+        rewrite (success_t2l empty)//=.
+        rewrite make_lB01_empty2; repeat split => //.
+        have [?] := s2l_Expanded_call vB eB H1; subst.
         case X: F => [?[|[sz z]zs]].
           move=> [Hm Hn].
           by rewrite Hn//clean_ca_cat//cat0s.
@@ -274,27 +195,24 @@ Section next_callS.
         rewrite !clean_ca_cat /save_alts map_cons !catA !cat_cons; repeat f_equal.
           rewrite clean_ca_save_goals//=?clean_ca_cat//=.
           by apply: empty_ca_atoms.
-        (* rewrite -/(save_alts ((xs ++ ml) ++ bt) gs (aa2gs zs)). *)
-        (* rewrite -/(save_alts (append_alts (clean_ca bt xs) (clean_ca bt ml)) (clean_ca_goals bt gs) (aa2gs zs)). *)
         rewrite clean_ca_save_alts?empty_ca_atoms1//.
         by rewrite clean_ca_cat//.
       have [s2'[x[xs H]]] := failed_t2l vA fA s1 bt.
-      (* have [hd H1]:= base_and_t2l bB.
-      have E := base_and_empty_ca bB H1. *)
       rewrite H/= t2l_big_and => -[?+?]; subst.
       case: x H => //=.
         move=> H.
         exfalso.
         by apply: s2l_empty_hdF H.
       move=> [[|g] ign'] gs H [???]//; subst.
-      have /={HA} := HA s1 bt _ _ _ _ _ fA vA _.
-      rewrite H/= => /(_ _ _ _ _ _ erefl) [He + H3].
-      rewrite what_I_want?(next_callS_valid _ _ erefl)// => H2.
-      rewrite H3; repeat split => //.
-      have [?] := s2l_Expanded_call vA H3 H; subst.
+      have /={HA HB} := HA s1 bt _ _ _ _ _ fv fA vA.
+      rewrite H/= => /(_ _ _ _ _ _ erefl)[].
+      rewrite eA => /= + [??]; subst => /=.
+      rewrite (what_I_want (valid_tree_step vA eA)) => /=H2.
+      split => //.
+      rewrite seq2altsK seq2goals_cat !seq2goalsK.
+      have [?] := s2l_Expanded_call vA eA H; subst.
       rewrite push.
       have?:= empty_caG_r2l.
-      rewrite seq2altsK.
       case X: F => [?[|[sz z]zs]][?]; subst.
         move=> [Hm Hn]; subst.
         case W: t2l => //=[[sw w]ws].
@@ -303,10 +221,10 @@ Section next_callS.
         by rewrite clean_ca_mk_lb0//=.
       move=> [Hm Hn]; rewrite Hn/=.
       rewrite t2l_big_and.
-      rewrite !clean_ca_goals_cat/=.
+      rewrite !clean_ca_goals_cat/= seq2altsK.
       set hd := (r2l B0).
       have E : empty_caG hd by apply: empty_caG_r2l.
-      rewrite -{2}(cat0s bt) seq2altsK.
+      rewrite -{2}(cat0s bt).
       have HH := @clean_ca_add_deep_gs no_alt bt hd gs E.
       rewrite cat0s in HH.
       rewrite HH clean_ca_goals_cat.
